TheologExercises2026/Exercises/Exercise02.lean
@@ -265,28 +265,6 @@ def NNFFormula.KNF (F : NNFFormula Atom) : NNFFormula Atom :=
 theorem NNFFormula.DNF_and (G H : NNFFormula Atom) : (NNFFormula.and G H).isDNF ↔ G.onlyAnd ∧ H.onlyAnd := by
   unfold isDNF; grind
 
-theorem NNFFormula.DNF_isDNF (F : NNFFormula Atom) : F.DNF.isDNF := by
-  induction F with
-  | and F1 F2 h1 h2 =>
-    unfold isDNF-- DNF DNF.loop
-    cases h : (F1.and F2).DNF with
-    | and G1 G2 =>
-      simp only [Bool.and_eq_true]
-      constructor
-      . unfold DNF DNF.loop at h
-
-        sorry
-      . sorry
-    | or G1 G2 =>
-      simp only [Bool.and_eq_true]
-
-      sorry
-    | _ => grind
-  | or F1 F2 h1 h2 =>
-    unfold isDNF
-    sorry
-  | _ => sorry
-
 def F := ⟪ (¬("p" ∨ "q") ∧ (("r" ∨ (¬"q" ∨ "p"))) ∧ "p") ⟫
 def G := ⟪ "p" ∧ ("q" ∧ (¬"q" ∨ "p")) ⟫
 
@@ -300,124 +278,6 @@ def G := ⟪ "p" ∧ ("q" ∧ (¬"q" ∨ "p")) ⟫
 
 #eval ⟪ ("x" → ("p" → "q") → "r" ) ⟫.to_only_andornot.toFormula
 #eval ⟪ ("x" → ("p" → "q") → "r" ) ⟫.to_only_andornot.toNNF.toFormula
-
-theorem Formula.de_morgan1 (F G : Formula Atom) : ⟪ ¬(F ∧ G) ⟫ === ⟪ ¬F ∨ ¬G ⟫ := by intro v; grind
-theorem Formula.de_morgan2 (F G : Formula Atom) : ⟪ ¬(F ∨ G) ⟫ === ⟪ ¬F ∧ ¬G ⟫ := by intro v; grind
-
-theorem Formula.not_equiv_of_equiv (F G : Formula Atom) : F === G -> F.not === G.not := by
-  intro equiv v
-  unfold Valuation.eval
-  specialize equiv v
-  grind
-
-theorem Formula.eq_onlyAndOrNot : ∀ (F : Formula Atom), F === F.to_only_andornot.toFormula := by
-  intro F
-  unfold equiv
-  intro v
-  induction F with
-  | atom p => simp only [to_only_andornot, OnlyAndOrNotFormula.toFormula]
-  | not F => simp only [to_only_andornot, OnlyAndOrNotFormula.toFormula]; grind
-  | and F G h1 h2 => simp only [to_only_andornot, OnlyAndOrNotFormula.toFormula]; grind
-  | or F G h1 h2 => simp only [to_only_andornot, OnlyAndOrNotFormula.toFormula]; grind
-  | imp F G h1 h2 => simp only [to_only_andornot, OnlyAndOrNotFormula.toFormula]; grind
-  | eq F G h1 h2 => simp only [to_only_andornot, OnlyAndOrNotFormula.toFormula]; grind
-  | _ => simp only [to_only_andornot, OnlyAndOrNotFormula.toFormula]
-
-theorem test (F G : OnlyAndOrNotFormula Atom) : (F.and G).toFormula === (F.and G).toNNF.toFormula -> (F.and G).not.toFormula === (F.and G).not.toNNF.toFormula := by
-  intro equiv v
-  specialize equiv v
-  have aux : v.eval (F.and G).not.toFormula = v.eval (F.and G).toFormula.not := by rfl
-  --have aux2 : v.eval (F.and G).not.toNNF.toFormula = v.eval (F.and G).toNNF.toFormula.not := by sorry
-  simp only [aux, Valuation.eval]--, equiv]
-  apply Classical.byContradiction
-  intro contra
-  simp at contra
-
-  sorry
-
-theorem Formula.not_eq_not_NNF (F : Formula Atom) : F === F.to_only_andornot.toNNF.toFormula → ⟪ ¬F ⟫ === ⟪ ¬F ⟫.to_only_andornot.toNNF.toFormula := by
-  intro equiv v
-  induction F with
-  | top =>
-    simp only [to_only_andornot, OnlyAndOrNotFormula.toNNF]
-    unfold Valuation.eval NNFFormula.toFormula
-    simp only
-    rfl
-  | bot =>
-    simp only [to_only_andornot, OnlyAndOrNotFormula.toNNF]
-    unfold Valuation.eval NNFFormula.toFormula
-    simp only
-    rfl
-  | atom p =>
-    simp only [to_only_andornot, OnlyAndOrNotFormula.toNNF]
-    rfl
-  | and F1 F2 h1 h2 =>
-    simp only [to_only_andornot, OnlyAndOrNotFormula.toNNF, Valuation.eval]
-    sorry
-  | _ =>
-    sorry
-
-theorem Formula.eq_NNF (F : Formula Atom) : F === F.to_only_andornot.toNNF.toFormula := by
-  unfold equiv
-  intro v
-  rw [eq_onlyAndOrNot]
-  induction F with
-  | top => simp only [to_only_andornot, OnlyAndOrNotFormula.toFormula, OnlyAndOrNotFormula.toNNF]; rfl
-  | bot => simp only [to_only_andornot, OnlyAndOrNotFormula.toFormula, OnlyAndOrNotFormula.toNNF]; rfl
-  | atom p => simp only [to_only_andornot, OnlyAndOrNotFormula.toFormula, OnlyAndOrNotFormula.toNNF]; rfl
-  | not F h =>
-    simp only [to_only_andornot, OnlyAndOrNotFormula.toFormula, Valuation.eval, Bool.not_eq_eq_eq_not, h]
-
-    sorry
-  | and F G h1 h2 =>
-    simp only [to_only_andornot, OnlyAndOrNotFormula.toFormula, OnlyAndOrNotFormula.toNNF, Valuation.eval, h1, h2]
-    rfl
-  | or F G h1 h2 =>
-    simp only [to_only_andornot, OnlyAndOrNotFormula.toFormula, OnlyAndOrNotFormula.toNNF, Valuation.eval, h1, h2]
-    rfl
-  | imp F G h1 h2 =>
-    simp only [to_only_andornot, OnlyAndOrNotFormula.toFormula, OnlyAndOrNotFormula.toNNF]--, Valuation.eval, h1, h2]
-
-    sorry
-  | eq F G h1 h2 =>
-    simp only [to_only_andornot, OnlyAndOrNotFormula.toFormula, OnlyAndOrNotFormula.toNNF, Valuation.eval, h1, h2]
-
-    sorry
-
-theorem OnlyAndOrNotFormula.eq_NNF' (F : OnlyAndOrNotFormula Atom) : F.toFormula === F.toNNF.toFormula := by
-  unfold Formula.equiv
-  intro v
-  induction F with
-  | top =>
-    simp only [toFormula, toNNF, NNFFormula.toFormula]
-  | bot => simp only [toFormula, toNNF, NNFFormula.toFormula]
-  | atom => simp only [toFormula, toNNF, NNFFormula.toFormula]
-  | and => simp only [toFormula, toNNF, NNFFormula.toFormula, Valuation.eval]; grind
-  | or => simp only [toFormula, toNNF, NNFFormula.toFormula, Valuation.eval]; grind
-  | not G ih =>
-    --simp only [toFormula, Valuation.eval]
-    induction hG : G with
-    | top => sorry
-    | bot => sorry
-    | atom => sorry
-    | and G1 G2 h1 h2 =>
-      simp only [toNNF, toFormula]
-      rw [Formula.de_morgan1]
-      rw [hG] at ih
-      have aux : (G1.not.and G2.not).toNNF = G1.not.toNNF.and G2.not.toNNF := by
-        conv =>
-          lhs
-          unfold toNNF
-
-
-
-
-      sorry
-    | _ =>
-      sorry
-
-theorem Formula.eq_DNF (F : Formula Atom) : F === F.to_only_andornot.toNNF.DNF.toFormula := by sorry
-
 
 section Exercise02
 
@@ -464,18 +324,3 @@ def F_d := ⟪ ¬("c" → ((¬"a" ∧ "b" ∧ "c") ∨ ("a" ∧ ¬"b"))) ⟫
 
 end Exercise02
 
-
-namespace NNFFormula
-
-def atoms : NNFFormula Atom -> List Atom
-| .atom p => [p]
-| .negatom p => [p]
-| .or F G => F.atoms ++ G.atoms
-| .and F G => F.atoms ++ G.atoms
-| _ => []
-
-def new_atom (F : NNFFormula Nat) : Nat := match F.atoms with
-| [] => 0
-| a::l => (a::l).max (by grind) + 1
-
-end NNFFormula
