TheologExercises2026/WorkInProgress/UnitPropagation.lean
@@ -1,0 +1,139 @@
+import TheologExercises2026.Exercises.Exercise04
+
+theorem HornFormula.sat_iff_unit_sat [DecidableEq Atom] (H : HornFormula Atom) (L : HornClause Atom) : H.toFormula.satisfiable ↔ (H.unit L).toFormula.satisfiable := by
+  unfold Formula.satisfiable
+  constructor
+  . intro sat
+    rcases sat with ⟨v, v_sat⟩
+    exists v
+    unfold unit
+    rw [eval_toFormula_eq] at *
+    by_cases L_mem : L ∈ H
+    . simp only [L_mem, if_true]
+      . split
+        -- neg. unit clause
+        next hd body p hd_eq body_eq =>
+          simp?
+          intro C C_mem
+          by_cases hC : C.body.contains p
+          . apply Or.inl; grind
+          . apply Or.inr
+            have C_eval : v.eval C.toFormula = true := by grind
+            simp at hC
+            rw [HornClause.eval_true_iff] at C_eval
+            have test := (HornClause.eval_true_iff (C.remove p) v).mpr
+            rcases C_eval with ⟨q, hq⟩
+            have aux : ∃ q, (C.remove p).head.isEqSome q = true ∧ v.eval (Formula.atom q) = true ∨ q ∈ (C.remove p).body ∧ v.eval (Formula.atom q) = false := by
+              exists q
+              apply Or.inr
+              constructor
+              .
+                sorry
+              . sorry
+
+
+            --rcases C_eval with ⟨q, ⟨q_hd, q_eval⟩ | ⟨q_mem, q_eval⟩⟩
+
+            sorry
+        next hd body p hd_eq body_eq =>
+          simp
+          intro C C_mem
+          by_cases hC : C.head == some p
+          . apply Or.inl; grind
+          . apply Or.inr
+            simp only [Bool.not_eq_true] at hC
+            have C_eval : v.eval C.toFormula := by grind
+            have p_eval : v.eval (Formula.atom p) := by
+              simp only [List.all_eq, List.mem_map, forall_exists_index, and_imp, forall_apply_eq_imp_iff₂,decide_eq_true_eq] at v_sat
+              specialize v_sat L L_mem
+              unfold HornClause.toFormula at v_sat
+              simp [hd_eq, body_eq, Formula.disjunction_from_list] at v_sat
+              exact v_sat
+            have not_p_eval : !v.eval (Formula.atom p).not := by grind
+            have test := (HornClause.eval_true_iff C v).mp C_eval
+
+            unfold HornClause.remove
+            simp only [Option.isEqSome_eq_beq_some, hC, Bool.false_eq_true, ↓reduceIte]
+            cases C_head : C.head with
+            | none =>
+              rcases test with ⟨q, ⟨q_hd, q_eval⟩ | ⟨q_mem, q_eval⟩⟩
+              . grind
+              . have q_mem' : q ∈ C.body.removeAll [p] := by grind
+                rw [HornClause.eval_true_iff]
+                exists q
+                simp; exact ⟨q_mem', q_eval⟩
+            | some r =>
+              rcases test with ⟨q, ⟨q_hd, q_eval⟩ | ⟨q_mem, q_eval⟩⟩
+              . unfold HornClause.toFormula Formula.disjunction_from_list
+                simp only; grind
+              . have q_mem' : q ∈ C.body.removeAll [p] := by grind
+                rw [HornClause.eval_true_iff]
+                exists q
+                simp only [Option.isEqSome_eq_beq_some, Option.some_beq_some, beq_iff_eq]
+                apply Or.inr
+                exact ⟨q_mem', q_eval⟩
+        . grind
+    . simp only [L_mem, if_false]; grind
+
+  . rintro ⟨v, v_eval⟩
+    by_cases L_mem : L ∈ H
+    . simp only [unit, L_mem, if_true] at v_eval
+      split at v_eval
+      next hd body p L_hd L_body =>
+        let v' : Valuation Atom := fun x => if x == p then false else v x
+        exists v'
+        rw [eval_toFormula_eq] at *
+        simp only [List.all_map, List.all_eq_true, Function.comp_apply] at *
+        simp only [List.elem_eq_contains, List.contains_eq_mem, List.mem_filter, Bool.not_eq_eq_eq_not, Bool.not_true, decide_eq_false_iff_not, and_imp] at v_eval
+        intro C C_mem
+        by_cases p_mem : p ∈ C.body
+        . rw [HornClause.eval_true_iff]
+          exists p
+          apply Or.inr
+          constructor
+          . exact p_mem
+          . unfold v'
+            grind
+        . specialize v_eval C C_mem p_mem
+          rw [HornClause.eval_true_iff] at v_eval
+          have p_nmem : ¬p ∈ C.remove p := by
+            unfold HornClause.remove Membership.mem HornClause.instMembership
+            simp only [List.removeAll]
+            simp only [Option.isEqSome_eq_beq_some, beq_iff_eq, Option.ite_none_left_eq_some, not_and_self, List.contains_eq_mem, List.not_mem_nil, or_false,
+              List.decide_mem_cons, decide_false, Bool.or_false, List.mem_filter, BEq.rfl, Bool.not_true, Bool.false_eq_true, and_false, not_false_eq_true]
+          have p_eval : v'.eval (Formula.atom p) = false := by grind
+          rcases v_eval with ⟨q, v_eval⟩
+          rcases v_eval with ⟨q_hd, q_eval⟩ | ⟨q_mem, q_eval⟩
+          . rw [HornClause.eval_true_iff]
+            exists q
+            apply Or.inl
+            constructor
+            . unfold HornClause.remove at q_hd
+              simp only [Option.isEqSome_eq_beq_some, beq_iff_eq, Option.ite_none_left_eq_some] at *
+              exact q_hd.right
+            . have q_mem : q ∈ C.remove p := by
+                unfold Membership.mem HornClause.instMembership
+                simp only [Option.isEqSome_eq_beq_some, beq_iff_eq] at q_hd
+                apply Or.inl
+                exact q_hd
+              have q_neq : q ≠ p := by grind
+              grind
+          . rw [HornClause.eval_true_iff]
+            exists q
+            apply Or.inr
+            constructor
+            . unfold HornClause.remove at q_mem
+              simp only at q_mem
+              grind
+            . grind
+      next hd body p L_hd L_body =>
+        let v' : Valuation Atom := fun x => if x == p then true else v x
+        exists v'
+        rw [eval_toFormula_eq] at *
+        simp only [Option.isEqSome_eq_beq_some, List.map_map, List.all_map, List.all_filter, Bool.not_not, Function.comp_apply, List.all_eq_true, Bool.or_eq_true, beq_iff_eq] at *
+        intro C C_mem
+
+        sorry
+      next => grind
+    . simp only [unit, L_mem, if_false] at v_eval; exists v
+
